ModularEngine/src/LogicEngine.FStar.Wrapper/wrapper.fs
@@ -25,7 +25,7 @@ type substitution = Dictionary<Types.var, Types.term>
 
 type Wrapper() =
   
-  let rec PrimsListofList (l:list<'a>) : Prims.list<'a> = 
+  (*let rec PrimsListofList (l:list<'a>) : Prims.list<'a> = 
     match l with
     | [] -> new Prims.Nil<'a>() :> Prims.list<'a>
     | h::t -> new Prims.Cons<'a>(h, PrimsListofList t) :> Prims.list<'a>
@@ -34,7 +34,7 @@ type Wrapper() =
     match o with
     | None -> new Prims.None<'a>() :> Prims.option<'a>
     | Some(a) -> new Prims.Some<'a>(a) :> Prims.option<'a>
-  
+  *)
   let _signatureProvider: ISignatureProvider option ref = ref None
   let _infostrate: IInfostrate option ref = ref None
 
@@ -56,23 +56,30 @@ type Wrapper() =
       (!_signatureProvider).Value
 
     member le.Derive (target: ITerm) (substs: ISubstitution seq) : ISubstitution seq = 
-      substs |> List.ofSeq |> List.map TranslationToFStar.FStarSubstitutionOfISubstitution |>
-      PrimsListofList |>
-      LogicEngine.deriveWrapper (PrimsOptionofOption !_infostrate) (TranslationToFStar.FStarTermOfITerm target) |>
+      substs |> List.ofSeq |>
+      List.map TranslationToFStar.FStarSubstitutionOfISubstitution |>
+      Builders.PrimsListOfList |> 
+      InfonLogic.deriveWrapper 
+        (!_infostrate |> Option.map (fun i -> i.Knowledge |> Seq.toList 
+                                              |> List.map TranslationToFStar.FStarPolyTermOfITerm
+                                              |> Builders.PrimsListOfList)
+                      |> Builders.PrimsOptionOfOption)
+        (TranslationToFStar.FStarTermOfITerm target) |>
       List.map TranslationFromFStar.ISubstitutionOfFStarSubstitution |>
       Seq.ofList
 
     member le.DeriveJustification (infon: ITerm) (proofTemplate: ITerm) (substs: ISubstitution seq) =
       substs |> List.ofSeq |> List.map TranslationToFStar.FStarSubstitutionOfISubstitution |>
-      PrimsListofList |>
-      LogicEngine.deriveJustificationWrapper
-        (PrimsOptionofOption !_infostrate) (TranslationToFStar.FStarTermOfITerm infon) (TranslationToFStar.FStarTermOfITerm proofTemplate) |>
+      Builders.PrimsListOfList |>
+      InfonLogic.deriveJustificationWrapper
+        (Builders.PrimsOptionOfOption !_infostrate) (TranslationToFStar.FStarTermOfITerm infon) (TranslationToFStar.FStarTermOfITerm proofTemplate) |>
       List.map TranslationFromFStar.ISubstitutionOfFStarSubstitution |>
       Seq.ofList
 
     member le.CheckJustification (evidence: ITerm) =
-      //
-      evidence  |> TranslationToFStar.FStarTermOfITerm |>
-      LogicEngine.checkJustificationWrapper (Builders.PrimsOptionOfOption !_signatureProvider) |>
-      Option.map TranslationFromFStar.ITermOfFStarTerm
+      (*evidence  |> TranslationToFStar.FStarTermOfITerm |>
+      InfonLogic.checkJustificationWrapper 
+        (Builders.PrimsOptionOfOption !_signatureProvider) |>
+      Option.map TranslationFromFStar.ITermOfFStarTerm*)
+      failwith "TODO checkJustification"
 
